Define dependencies and generation of WFG from deps.

DependencyState.v
@@ -1,6 +1,11 @@
+(**
+  This module defines a resource dependency state, which is easily mapped
+  to a GRG. We define a function to generate a WFG from some
+  [dependencies]. *)
+
 Require Import Vars.
 Require Import ResourceDependency.
-Require Import Semantics.
+Require Import Project.
 
 Set Implicit Arguments.
 
@@ -19,89 +24,167 @@ Definition get_impedes (d:dependencies) : impedes := fst d.
 Definition WDep (w:waits) (t:tid) (r:resource) :=
   exists rs, Map_TID.MapsTo t rs w /\ Set_RES.In r rs.
 
-(** We build the phaser map of waiting tasks to be constituted by all
-   blocked tasks in state [s]. *)
-Definition W_of (s:state) (w:waits) := forall t r, WDep w t r <-> WaitsFor s t r.
+Definition WEdge d := (WDep (get_waits d)).
 
-(** A resource [r] impedes a task [r] if task [t] is registered in a
-   preceeding resource; the impeding resource must be the target of
-   a blocked task. *)
 
 (* An i-edge is an edge in the dependency state such that `t in I(t)`. *)
 Definition IDep (i:impedes) (r:resource) (t:tid) :=
   exists ts, Map_RES.MapsTo r ts i /\ Set_TID.In t ts.
 
-(** The map of impedes holds all resources that are blocking a task. *)
-Definition I_of (s:state) (i:impedes) := forall t r, IDep i r t <-> Impedes s r t.
+Definition IEdge d := (IDep (get_impedes d)).
 
-Definition Deps_of (s:state) (d:dependencies) := W_of s (get_waits d) /\ I_of s (get_impedes d).
+(**
+  
+  In this section we define the construction of a WFG from a totally deadlocked
+  state. More precisely, by definition of [TotallyDeadlocked], every [t] waits
+  for some [r] and this [r] impedes some [t'], hence there is an outgoing
+  WFG-edge from [t] to [t']. Theorem [all_pos_odegree_impl_cycle] states
+  that a finite graph in which all vertices have outgoing edges includes a cycle.
+  To prove this result we need to provide a WFG defined as a list of pairs
+  of [tid]s that represent the WFG-edges.
+  
+  The goal of this section is to define an algorithm that constructs a
+  WFG from a given [state]. The translation from [state]s into WFG proceeds in
+  two steps: first, by converting [state]s into [dependencies];
+  and then by converting [depedencies] into the WFG. The conversion from
+  a [state] into [dependencies] is handled by Theorem [deps_of_total], so in
+  this section we only define the second step of translation.
+  *)
 
-Notation WEdge d := (WDep (get_waits d)).
-Notation IEdge d := (IDep (get_impedes d)).
+(** The [Project] module converts maps of sets into list of pairs. Let [I_Proj]
+    for maps of type [impedes]. *)
 
-Section Basic.
-  Variable d:dependencies.
-  Variable s:state.
-  Variable d_of_s: Deps_of s d.
+Module I_Proj := Project.Project Map_RES Set_TID.
+(** Function [impedes_edges] converts a map of [impedes] relation into
+    a list of pairs. *)
+Definition impedes_edges : impedes -> list (resource * tid) := I_Proj.edges.
 
-Let wedge_to_waits_for:
-  forall r t,
-  WEdge d t r ->
-  WaitsFor s t r.
+(** Lemma [impedes_edges_spec] establishes the correctness of
+    Function [impedes_edges]: each pair in the outcome of the
+    function is in relation [IEdge].
+    
+    To prove this result we use Lemma [Project.edges_spec]. *)
+Lemma impedes_edges_spec:
+  forall r t d,
+  List.In (r,t) (impedes_edges (get_impedes d)) <-> IEdge d r t.
 Proof.
   intros.
-  unfold WDep in H.
-  assert (H':= d_of_s).
-  destruct H' as (H', _).
-  apply H' in H.
-  assumption.
-Qed.
-
-Let waits_for_to_wedge:
-  forall r t,
-  WaitsFor s t r ->
-  WEdge d t r.
-Proof.
-  intros.
-  unfold WDep in *.
-  assert (H':= d_of_s).
-  destruct H' as (H', _).
-  apply H' in H.
-  assumption.
-Qed.
-
-(** If we have that [d] are the state-depencies of
-    a state [s], then a W-edge is equivalent to a waits-for
-    relation. *)
-Lemma wedge_eq_waits_for:
-  forall r t,
-  WEdge d t r <-> WaitsFor s t r.
-Proof.
-  intros.
-  split.
-  apply wedge_to_waits_for.
-  apply waits_for_to_wedge.
-Qed.
-
-(** Similarly, an i-edge is equivalent to an impedes relation. *)
-Lemma iedge_eq_impedes:
-  forall r t,
-  IEdge d r t <-> Impedes s r t.
-Proof.
-  intros.
-  split.
-  - intros.
-    unfold IDep in *.
-    assert (H':= d_of_s).
-    destruct H' as (_, H').
-    apply H'.
+  unfold IDep.
+  unfold impedes_edges.
+  apply I_Proj.edges_spec.
+  - intros. destruct H, k1, k2.
     auto.
-  - intros.
-    unfold IDep.
-    assert (H':= d_of_s).
-    destruct H' as (_, H').
-    apply H'.
-    assumption.
+  - auto.
 Qed.
 
-End Basic.
+(** Similarly, we project the map I into pairs of tasks and resources. *)
+Module W_Proj := Project.Project Map_TID Set_RES.
+Definition waits_edges : waits -> list (tid * resource) := W_Proj.edges.
+(** By using lemma [Project.edges_spec], we get that any pair
+    in [waits_edges] is a [WEdge] (aka impedes relation). *)
+Lemma waits_edges_spec:
+  forall t r d,
+  List.In (t,r) (waits_edges (get_waits d)) <-> WEdge d t r.
+Proof.
+  intros.
+  unfold waits_edges.
+  unfold WDep.
+  apply W_Proj.edges_spec.
+  - auto.
+  - intros. destruct H, e1, e2.
+    auto.
+Qed.
+
+Require Import Coq.Lists.List.
+
+Definition WFGEdge d t t' := exists r, WEdge d t r /\ IEdge d r t'.
+
+(** Given the impedes of a dependency state [d], filter the edges
+    matching [r]. *)
+Definition impedes_matching d r := 
+  filter
+  (fun e:(resource*tid)=>
+    let (r', t) := e in
+    if RES.eq_dec r' r then true else false)
+  (impedes_edges (get_impedes d)).
+(** Given a task [t] waiting for resource [r], compute WEdges starting
+    from [t]. The definition uses function [impedes_matching]. *)
+Definition build_edges (d:dependencies) (e:(tid*resource)) : list (tid*tid) :=
+  let (t, r) := e in
+  map (fun e':(resource*tid)=> (t, snd e')) (impedes_matching d r).
+(** For each blocked tasks in the dependency state compute the WEdges
+    using function [build_edges].*)
+Definition build_wfg (d:dependencies) : list (tid*tid) :=
+  flat_map (build_edges d) (waits_edges (get_waits d)).
+(** The first main result is to show that any pair in
+     [build_wfg] is a [WEdge]. The proof uses lemmas
+     [waits_edges_spec] and [impedes_edges_spec]. *)
+Theorem build_wfg_spec:
+  forall d t t',
+  List.In (t,t') (build_wfg d) <-> WFGEdge d t t'.
+Proof.
+  intros.
+  unfold build_wfg.
+  rewrite in_flat_map.
+  unfold build_edges in *.
+  split.
+  - intros.
+    (* We have that there exists a (t1, r) in [wait_edges]. *)
+    destruct H as ((t1, r), (Hinw, Hinb)).
+    rewrite waits_edges_spec in Hinw.
+    (* Thus, we have that (t1, r) is a [WEdge]. *)
+    exists r.
+    rewrite in_map_iff in *.
+    destruct Hinb as ((r', t''), (Heq, Hini)).
+    simpl in *.
+    inversion Heq; subst; clear Heq.
+    (* We also know that (r', t') is in [impedes_matching d r]. *)
+    unfold impedes_matching in *.
+    rewrite filter_In in *.
+    destruct Hini as (Hini, Hcnd).
+    remember (Map_RES_Extra.P.F.eq_dec r' r) as b.
+    destruct b.
+    assert (r' = r).
+    destruct a, r', r.
+    auto.
+    subst.
+    clear a Heqb.
+    rewrite impedes_edges_spec in *.
+    intuition.
+    inversion Hcnd.
+  - intros.
+    destruct H as (r, (Hwf, Him)).
+    exists (t, r).
+    rewrite waits_edges_spec.
+    intuition.
+    rewrite in_map_iff.
+    exists (r, t').
+    simpl.
+    intuition.
+    unfold impedes_matching.
+    rewrite filter_In.
+    split.
+    * rewrite impedes_edges_spec.
+      assumption.
+    * destruct (Map_RES_Extra.P.F.eq_dec r r).
+      auto.
+      contradiction n.
+      auto.
+Qed.
+
+(** Let [WFG_of] be the definition of a finite WFG defined
+    as a sequence of edges. *)
+Definition WFG_of d wfg := 
+  forall t t', List.In (t, t') wfg <-> WFGEdge d t t'.
+(** Given [build_wfg_spec] it is easy to show that we can
+    always obtain a finite WFG from a dependency state [d].*)
+Corollary wfg_of_total:
+  forall d:dependencies, exists wfg, WFG_of d wfg.
+Proof.
+  intros.
+  unfold WFG_of.
+  exists (build_wfg d).
+  intros.
+  rewrite build_wfg_spec.
+  auto with *.
+Qed.
